lib/file.ml
@@ -1,0 +1,9 @@
+type file_descriptor = Unix.file_descr
+
+let open_file path = Unix.openfile (Bytestring.to_string path) [ O_RDONLY ] 0
+
+let file_exists path = Bytestring.to_string path |> Sys.file_exists
+
+let read fd = ExtUnix.read_all_from ~line:false fd |> Bytestring.of_string
+
+let close = Unix.close
