lib/file.mli
@@ -1,0 +1,6 @@
+type file_descriptor = Unix.file_descr
+
+val open_file : Bytestring.t -> file_descriptor [@@impure]
+val file_exists : Bytestring.t -> bool [@@impure]
+val read : file_descriptor -> Bytestring.t [@@impure]
+val close : file_descriptor -> unit [@@impure]
