lib/log.ml
@@ -1,0 +1,3 @@
+open Coqbase
+
+let echo msg = print_string @@ Bytestring.to_string msg
