lib/log.mli
@@ -1,0 +1,3 @@
+open Coqbase
+
+val echo : Bytestring.t -> unit [@@impure]
