lib/tcp.ml
@@ -1,0 +1,29 @@
+open ExtUnix
+
+type socket_descriptor = Unix.file_descr
+
+let parse_address addr =
+  match Str.(split (regexp ":") addr) with
+  | [hostname; port] -> (Unix.inet_addr_of_string hostname, int_of_string port)
+  | _ -> failwith "Invalid address"
+
+let new_tcp_socket addr =
+  let hostname, port = parse_address (Bytestring.to_string addr) in
+  let fd = Unix.(socket PF_INET SOCK_STREAM 0) in
+  Unix.setsockopt fd SO_REUSEADDR true;
+  Unix.(bind fd (ADDR_INET (hostname, port)));
+  fd
+
+let listen_incoming_connection socket =
+  Unix.listen socket 1
+
+let read_socket socket = read_all_from socket |> Bytestring.of_string
+
+let write_socket socket data =
+  write_all_to socket (Bytes.of_string @@ Bytestring.to_string data)
+
+let close_socket socket = Unix.close socket
+
+let accept_connection socket =
+  let new_socket, _ = Unix.accept socket in
+  new_socket
