lib/tcp.mli
@@ -1,0 +1,8 @@
+type socket_descriptor = Unix.file_descr
+
+val new_tcp_socket : Bytestring.t -> socket_descriptor [@@impure]
+val listen_incoming_connection : socket_descriptor -> unit [@@impure]
+val read_socket : socket_descriptor -> Bytestring.t [@@impure]
+val write_socket : socket_descriptor -> Bytestring.t -> unit [@@impure]
+val close_socket : socket_descriptor -> unit [@@impure]
+val accept_connection : socket_descriptor -> socket_descriptor [@@impure]
