plugin/TCP.ml
@@ -18,20 +18,18 @@
  * along with this program. If not, see <http://www.gnu.org/licenses/>.
  *)
 
-open Freespec_exec.Coqstr
+open Freespec_exec.Coqbytestring
 open Freespec_exec.Extends
 open Freespec_exec.Coqunit
-open ExtUnix
+open Minihttpserver_lib
 
 let path = "minihttpserver.tcp"
 
-let parse_address addr =
-  match Str.(split (regexp ":") addr) with
-  | [hostname; port] -> (Unix.inet_addr_of_string hostname, int_of_string port)
-  | _ -> failwith "Invalid address"
-
 let constr_of_socket socket =
   Constr.(of_kind (Int (Uint63.of_int (Obj.magic socket))))
+
+let of_coqstring s = bytestring_of_coqbytestring s
+let to_coqstring s = bytestring_to_coqbytestring s
 
 let socket_of_constr c =
   match Constr.kind c with
@@ -40,51 +38,35 @@ let socket_of_constr c =
 
 let new_tcp_socket = function
   | [addr] ->
-     let addr = string_of_coqbytes addr in
-     let hostname, port = parse_address addr in
-     let fd = Unix.(socket PF_INET SOCK_STREAM 0) in
-     Unix.setsockopt fd SO_REUSEADDR true;
-     Unix.(bind fd (ADDR_INET (hostname, port)));
-     constr_of_socket fd
+    of_coqstring addr |> Tcp.new_tcp_socket |> constr_of_socket
   | _ -> assert false
 
 let listen_incoming_connection = function
   | [socket] ->
-     Unix.listen (socket_of_constr socket) 1;
-     coqtt
+    socket_of_constr socket |> Tcp.listen_incoming_connection |> (fun _ -> coqtt)
   | _ -> assert false
 
 let accept_connection = function
   | [socket] ->
-     let new_socket, _ = Unix.accept (socket_of_constr socket) in
-     constr_of_socket new_socket
+    socket_of_constr socket |> Tcp.accept_connection |> constr_of_socket
   | _ -> assert false
 
 let read_socket = function
   | [socket] ->
-     read_all_from (socket_of_constr socket) |>
-     string_to_coqbytes
+     socket_of_constr socket |> Tcp.read_socket |> to_coqstring
   | _ ->
      assert false
 
-let write_all_from data fd =
-  let rec aux ofs len =
-    let n = Unix.write fd data ofs len in
-    if n < len then aux (ofs + n) (len - n)
-  in
-  aux 0 (Bytes.length data)
-
 let write_socket = function
   | [socket; str] ->
-     write_all_from (bytes_of_coqbytes str) (socket_of_constr socket);
+     Tcp.write_socket (socket_of_constr socket)  (of_coqstring str);
      coqtt
   | _ ->
      assert false
 
 let close_tcp_socket = function
   | [socket] ->
-     Unix.close (socket_of_constr socket);
-     coqtt
+    socket_of_constr socket |> Tcp.close_socket |> (fun _ -> coqtt)
   | _ ->
      assert false
 
