bin/Extract.v
@@ -1,0 +1,10 @@
+From Base Require Import Extraction.
+From FreeSpec.Core Require Import All Extraction.
+From FreeSpec.Stdlib Require Import Console.
+From MiniHTTPServer Require Import App.
+
+Timeout 2 Definition run_http_server : unit :=
+  let main := http_server 1000 in
+  gen_main main.
+
+Extraction "minihttpserver.ml" run_http_server.
