main.v
@@ -1,4 +1,4 @@
-From FreeSpec Require Import Exec.
+From FreeSpec Require Import Exec.All.
 From MiniHTTPServer Require Import App Exec.
 
 Exec (http_server 100).
