theories/Exec.v
@@ -1,8 +1,9 @@
-From FreeSpec Require Import Core Exec.
+From FreeSpec Require Import Core.All Exec.All.
 From MiniHTTPServer Require Import App.
 
+(*
 Register TCP as minihttpserver.tcp.type.
-Register NewTCPSocket as minihttpserver.tcp.NewTCPSocket.
+Register New_TCPSocket as minihttpserver.tcp.NewTCPSocket.
 Register ListenIncomingConnection as minihttpserver.tcp.ListenIncomingConnection.
 Register AcceptConnection as minihttpserver.tcp.AcceptConnection.
 Register ReadSocket as minihttpserver.tcp.ReadSocket.
@@ -15,7 +16,7 @@ Register FileExists as minihttpserver.filesystem.FileExists.
 Register Read as minihttpserver.filesystem.Read.
 Register Close as minihttpserver.filesystem.Close.
 
-Register EVAL as minihttpserver.eval.type.
-Register Eval as minihttpserver.eval.Eval.
-
+Declare ML Module "coqbase".
+Declare ML Module "minihttpserver_lib".
 Declare ML Module "minihttpserver_plugin".
+*)
