theories/Init.v
@@ -1,1 +1,4 @@
+From Base Require Export Prelude.
+From FreeSpec.Core Require Export All.
+
 Create HintDb minihttp.
